Implement proof of work. Mined first block!!

Extraction/src/Util.ml
@@ -1,10 +1,11 @@
 open Forests
 
 module Types = TypesImpl.TypesImpl
-module ConsensusParams = Impl.ProofOfWork
-module ForestImpl = Forests (Types) (ConsensusParams)
+module Consensus = Impl.ProofOfWork
+module ForestImpl = Forests (Types) (Consensus)
 
 open Types
+open Consensus
 
 let clist_to_string cl = String.concat "" (List.map (String.make 1) cl)
 let string_to_clist s = List.init (String.length s) (String.get s)
@@ -13,11 +14,13 @@ let string_of_tx tx = clist_to_string tx
 let string_of_hash h = clist_to_string h
 
 let string_of_block (b : coq_Block) =
-  let fmt = format_of_string "%s = {prev = %s, txs = %s}" in
+  let fmt = format_of_string "%s = {prev = %s, txs = %s, nonce = %s}" in
   Printf.sprintf fmt
-    (string_of_hash (ConsensusParams.hashB b))
-    (string_of_hash b.prevBlockHash)
+    (string_of_hash (hashB b))
+    (String.sub (string_of_hash b.prevBlockHash) 0 8)
     (String.concat " " (List.map string_of_tx b.txs))
+    (string_of_int b.proof)
 
 let string_of_blockchain (chain : coq_Blockchain) =
-  String.concat " " (List.map string_of_block chain)
+  String.concat "\n" (List.map string_of_block chain)
+
