Extraction/src/node.ml
@@ -4,24 +4,52 @@ open Util
 
 module Addr = Address.Addr
 module Types = TypesImpl.TypesImpl
-module ConsensusParams = Impl.ProofOfWork
-module ForestImpl = Forests (Types) (ConsensusParams)
-module ProtocolImpl = Protocol (Types) (ConsensusParams) (ForestImpl) (Addr)
+module Consensus = Impl.ProofOfWork
+module ForestImpl = Forests (Types) (Consensus)
+module Protocol = Protocol (Types) (Consensus) (ForestImpl) (Addr)
+
+let _ = Random.self_init ()
 
 let node_id = 0
-let st = ref (ProtocolImpl.coq_Init node_id);;
+let st = ref (Protocol.coq_Init node_id)
 
 open ForestImpl
 
+let mine (_ : unit )= 
+  let ts = ref (int_of_float (Unix.time ())) in
+  let found_block = ref false in
+  let new_state = ref !st in
+  let hashes = ref 0 in
+  while not (!found_block) do
+    let (st' , msgs) = Protocol.procInt !st Protocol.MintT !ts in
+    hashes := !hashes + 1 ;
+    if List.length msgs > 0 then
+      begin
+        found_block := true ;
+        new_state := st' ;
+      end
+  done;
+  Printf.printf "Found block after %s hashes!\n" (string_of_int !hashes) ;
+  !new_state
+
+
 let main () =
-  let chain = btChain !st.blockTree in
-  Printf.printf "Chain: %s\n" (string_of_blockchain chain) ;;
+  Printf.printf "You are node %s\n" (string_of_int !st.id) ;
 
   let blocks = all_blocks !st.blockTree in
   Printf.printf "Your blocktree has %s block(s)!\n"
-    (string_of_int (List.length blocks)) ;;
- 
-  Printf.printf "You are node %s\n" (string_of_int !st.id) ;;
+    (string_of_int (List.length blocks)) ;
+
+  let chain = btChain !st.blockTree in
+  Printf.printf "Chain:\n %s\n" (string_of_blockchain chain) ;
+
+
+  st := (mine ()) ;
+  Printf.printf "Chain:\n %s\n" (string_of_blockchain (btChain !st.blockTree)) ;
+  Printf.printf "Work of last block: %s\n"
+    (string_of_int
+      (Obj.magic (Consensus.work (List.nth (btChain !st.blockTree) 1)))
+    ) ;;
 
 let () = main ()
 
