Extraction/Impl.v
@@ -16,9 +16,9 @@ Module ProofOfWork <: (ConsensusParams TypesImpl).
 Import TypesImpl.
 
 Definition GenesisBlock : block :=
-  mkB ((of_N 0) <: Hash)
+  mkB (("0x6150cb353fe365318be1040f4f1d55ba6a6235c7fdee7e94602fed76f112f2de")%string <: Hash)
       [::]
-      (tt <: VProof).
+      ((N_of_nat 0) <: VProof).
 
 Definition subchain (bc1 bc2 : Blockchain) := exists p q, bc2 = p ++ bc1 ++ q.
 Definition bcLast (bc : Blockchain) := last GenesisBlock bc.
@@ -30,8 +30,44 @@ Parameter hashB : block -> Hash.
 Definition WorkAmnt := N_ordType.
 
 (* TODO: don't hardcode the length of the hash *)
+(* Keep in mind that N extracts to int. Make sure to not overflow!
+    e.g. (to_N (hashB b)) will immediately overflow
+ *)
+
+(* Lookup table; lz[i] = how many leading 0s does i have as a 4-bit binary number ? *)
+Let leading_zeroes : seq N :=
+  [:: 4; 3; 2; 2; 1; 1; 1; 1;
+      0; 0; 0; 0; 0; 0; 0; 0
+  ]%N .
+
+Fixpoint _cbzs (s : string) : N :=
+  match s with
+  | String c s =>
+        let d_opt := ascii_to_digit c in
+        match d_opt with
+        | None => N0
+        | Some d =>
+          let lz := (nth N0 leading_zeroes d) in
+          if lz == N_of_nat(4) then (lz + _cbzs s)%N else lz
+        end
+  | _ => N0
+  end.
+
+(* Given a hex string, count how many binary zeroes it starts with *)
+Definition count_binary_zeroes (s : string) : N :=
+  match s with
+  | String s0 (String so s)
+      => if ascii_dec s0 "0"
+        then if ascii_dec so "x"
+          then _cbzs s
+          else N0
+        else N0
+  | _ => N0
+  end.
+
 Definition work (b : block) : WorkAmnt :=
-  (256 - N.log2 (to_N (hashB b)))%N.
+  count_binary_zeroes (hashB b).
+
 Fixpoint total_work (bc : Blockchain) : N_ordType :=
   match bc with
   | b::bc' => (work b + total_work bc')%N
@@ -71,7 +107,7 @@ Definition VAF (b : Block) (bc : Blockchain) (tp : TxPool) : bool :=
   if (b == GenesisBlock) then
     if (bc == [::]) && (tp == [::]) then true else false
   (* All other blocks do *)
-  else if (16 <? (work b))%N then true else false.
+  else if (12 <? (work b))%N then true else false.
 
 (* For proof-of-work, this would be more aptly called "getNonce" *)
 (* TODO: Implement this in the extraction *)
